src/Examples/QueryStructure/IncompleteROSMaster.v
@@ -1,0 +1,722 @@
+Require Import Fiat.QueryStructure.Automation.MasterPlan.
+
+Definition int := nat.
+Definition ERROR := 2. (* should have been defined as -1 *)
+Definition FAILURE := 0.
+Definition SUCCESS := 1.
+
+Definition any := string.
+
+Definition sSUBSCRIPTIONS := "Subscriptions".
+Definition sPUBLICATIONS := "Publications".
+Definition sSERVICES := "Services".
+Definition sTOPICS := "Topics".
+Definition sTOPIC := "topic".
+Definition sNODE_ID := "node_id".
+Definition sNODE_API := "node_api".
+Definition sSERVICE_API := "service_api".
+Definition sSERVICE := "service".
+Definition sTOPIC_TYPE := "topic_type".
+Definition sNODES := "Nodes".
+Definition sPARAMS := "Parameters".
+Definition sKEY := "key".
+Definition sVALUE := "value".
+Definition sPARAMSUBSCRIPTIONS := "ParamSubscriptions".
+
+(* what happen if the same tuple is repeatedly inserted in sNODES? *)
+(* want drop it when the same thing comes in *)
+
+Definition DuplicateFree {heading} (tup1 tup2 : @RawTuple heading) := tup1 <> tup2.
+
+Fixpoint BuildFinUpTo (n : nat) {struct n} : list (Fin.t n) :=
+  match n return list (Fin.t n) with
+  | 0  => nil
+  | S n' => cons (@Fin.F1 _) (map (@Fin.FS _) (BuildFinUpTo n'))
+  end.
+
+Definition allAttributes heading
+  : list (Attributes heading) :=
+  BuildFinUpTo (NumAttr heading).
+
+Lemma refine_DuplicateFree
+      {qsSchema}
+  : forall (qs : UnConstrQueryStructure qsSchema) Ridx tup',
+    refine
+      {b : bool |
+       decides b
+               (forall tup : IndexedElement,
+                   GetUnConstrRelation qs Ridx tup ->
+                   DuplicateFree tup' (indexedElement tup))}
+      (xs <- For (UnConstrQuery_In qs Ridx
+                           (fun tup => Where (tupleAgree_computational tup' tup (allAttributes _) )
+                                             Return ()));
+       ret (if hd_error xs then true else false)).
+Proof.
+Admitted.
+
+Lemma refine_DuplicateFree_symmetry
+      {qsSchema}
+  : forall (qs : UnConstrQueryStructure qsSchema) Ridx tup' b',
+    computes_to {b : bool | decides b
+                                     (forall tup : IndexedElement,
+                                         GetUnConstrRelation qs Ridx tup ->
+                                         DuplicateFree tup' (indexedElement tup)  )} b'
+    -> refine
+         {b : bool |
+          decides b
+                  (forall tup : IndexedElement,
+                      GetUnConstrRelation qs Ridx tup ->
+                      DuplicateFree (indexedElement tup) tup')}
+         (ret b').
+Proof.
+Admitted.
+
+Ltac implement_DuplicateFree :=
+  match goal with
+    |- context [{b : bool |
+                 decides b
+                         (forall tup' : IndexedElement,
+                             GetUnConstrRelation ?r ?Ridx tup' ->
+                                 DuplicateFree ?tup (indexedElement tup'))}] =>
+    rewrite (@refine_DuplicateFree _ r Ridx)
+  end.
+
+Ltac implement_DuplicateFree_symmetry :=
+  match goal with
+    |- context [{b : bool |
+                 decides b
+                         (forall tup' : IndexedElement,
+                             GetUnConstrRelation ?r ?Ridx tup' ->
+                                 DuplicateFree  (indexedElement tup') ?tup)}] =>
+    rewrite (@refine_DuplicateFree_symmetry _ r Ridx)
+  end.
+
+
+Definition stringPrefix str str' : Prop :=
+  prefix str str' = true.
+
+Instance prefixDecideable {B} (f : B -> _) str'
+    : DecideableEnsemble (fun str => stringPrefix (f str) str')
+    := { dec str := prefix (f str) str'}.
+  intros.
+  unfold stringPrefix. destruct (prefix (f a) str'); simpl; split; eauto.
+Defined.
+
+Instance prefixDecideable' {B} (f : B -> _) str'
+  : DecideableEnsemble (fun str => stringPrefix str' (f str))
+    := { dec str := prefix str' (f str)}.
+  intros.
+  unfold stringPrefix. destruct (prefix str' (f a)); simpl; split; eauto.
+Defined.
+
+Ltac PickIndexes BuildEarlyIndex BuildLastIndex :=
+GenerateIndexesForAll
+   EqExpressionAttributeCounter
+   ltac:(fun attrlist =>
+           let attrlist' := eval compute in (PickIndexes _ (CountAttributes' attrlist)) in make_simple_indexes attrlist' BuildEarlyIndex BuildLastIndex).
+
+
+Ltac implement_nested_Query
+         CreateTerm EarlyIndex LastIndex
+         makeClause_dep EarlyIndex_dep LastIndex_dep :=
+    Focused_refine_Query;
+      [ match goal with
+    | [H : @DelegateToBag_AbsR ?qs_schema ?indexes ?r_o ?r_n
+       |- refine (UnConstrQuery_In (ResultT := ?resultT) ?r_o ?idx ?f) _ ] =>
+      etransitivity;
+        [ let H' := (eval simpl in (@refine_UnConstrQuery_In resultT _ r_o idx)) in
+          eapply H'; intro;
+          implement_Query CreateTerm EarlyIndex LastIndex
+                          makeClause_dep EarlyIndex_dep LastIndex_dep;
+          simpl; repeat first [setoid_rewrite refine_bind_unit
+                              | setoid_rewrite refine_bind_bind ];
+          simplify with monad laws; finish honing
+        | let H' := eval simpl in (refine_Filtered_Query_In_Enumerate (ResultT := resultT) H (idx := idx)) in
+              apply H']
+
+    end | ].
+
+
+    Lemma List_Query_In_Return' :
+      forall (n : nat) (ResultT : Type) (headings : Vector.t RawHeading n) (f f' : _ -> Comp (list ResultT))
+             (l : list (ilist2 (B := @RawTuple) headings)),
+        (forall tup, refine (f tup) (f' tup))
+        -> refine (List_Query_In l f)
+                  (List_Query_In l f').
+    Admitted.
+
+    Ltac Implement_Nested_Query_In :=
+      let r_o' := fresh "r_o'" in
+      let AbsR_r_o' := fresh "AbsR_r_o'" in
+      let refines_r_o' := fresh "refines_r_o'" in
+      match goal with
+      | H : @Build_IndexedQueryStructure_Impl_AbsR ?qs_schema ?Index ?DelegateReps ?DelegateImpls
+                                                   ?ValidImpls _ _
+        |- refine (Bind (List_Query_In ?l ?f) ?k) _ =>
+        setoid_rewrite (@List_Query_In_Return' _ _ _ f _ l);
+          [ | intros; repeat Implement_Bound_Bag_Call; finish honing];
+          setoid_rewrite List_Query_In_Return
+      end.
+
+    Ltac implement_bag_methods :=
+      etransitivity;
+      [ repeat (first [
+                    simpl; simplify with monad laws
+                  | remove_spurious_Dep_Type_BoundedIndex_nth_eq
+                  | Implement_If_Then_Else
+                  | Implement_If_Opt_Then_Else
+                  | Implement_Bound_Bag_Call
+                  | Implement_Bound_Join_Comp_Lists
+                  | Implement_Bound_Join_Comp_Lists'
+                  | Implement_AbsR_Relation
+                  | match goal with
+                      |- context[CallBagImplMethod _ _ _ _ _] =>
+                      unfold CallBagImplMethod; cbv beta; simpl
+                    end
+                  | Implement_Nested_Query_In
+                  | higher_order_reflexivity ]; simpl) |];
+      (* Clean up any leftover CallBagImplMethods *)
+      repeat (cbv beta; simpl;
+              match goal with
+                |- appcontext[CallBagImplMethod] =>
+                unfold CallBagImplMethod; cbv beta; simpl;
+                try remove_spurious_Dep_Type_BoundedIndex_nth_eq
+              end);
+      higher_order_reflexivity.
+
+
+Ltac FullySharpenQueryStructure'' qs_schema Index :=
+  let DelegateSigs := constr:(@Build_IndexedQueryStructure_Impl_Sigs _ (qschemaSchemas qs_schema) Index) in
+  let DelegateSpecs := constr:(@Build_IndexedQueryStructure_Impl_Specs _ (qschemaSchemas qs_schema) Index) in
+  let cRep' := constr:(@Build_IndexedQueryStructure_Impl_cRep _ (qschemaSchemas qs_schema) Index) in
+  let cAbsR' := constr:(@Build_IndexedQueryStructure_Impl_AbsR qs_schema Index) in
+  let ValidRefinements := fresh in
+  let FullySharpenedImpl := fresh "FullySharpenedImpl" in
+  match goal with
+    |- @FullySharpenedUnderDelegates _ (@BuildADT ?Rep ?n ?n' ?consSigs ?methSigs ?consDefs ?methDefs) _ =>
+    ilist_of_dep_evar n
+                      (Fin.t (numRawQSschemaSchemas qs_schema) -> Type)
+                      (fun D =>
+                         forall idx,
+                           ComputationalADT.pcADT (DelegateSigs idx) (D idx))
+                      (fun
+                          (DelegateReps : Fin.t _ -> Type)
+                          (DelegateImpls : forall idx,
+                              ComputationalADT.pcADT (DelegateSigs idx) (DelegateReps idx))
+                          (Sig : consSig) =>
+                          ComputationalADT.cConstructorType (cRep' DelegateReps)
+                                                            (consDom Sig))
+                      consSigs
+                      ltac:(fun cCons =>
+                              ilist_of_dep_evar n'
+                                                (Fin.t (numRawQSschemaSchemas qs_schema) -> Type)
+                                                (fun D =>
+                                                   forall idx,
+                                                     ComputationalADT.pcADT (DelegateSigs idx) (D idx))
+                                                (fun (DelegateReps : Fin.t _ -> Type)
+                                                     (DelegateImpls : forall idx,
+                                                         ComputationalADT.pcADT (DelegateSigs idx) (DelegateReps idx))
+                                                     (Sig : methSig) =>
+                                                   ComputationalADT.cMethodType (cRep' DelegateReps)
+                                                                                (methDom Sig) (methCod Sig))
+                                                methSigs
+                                                ltac:(fun cMeths =>
+                                                        assert
+                                                          ((forall
+                                                               (DelegateReps : Fin.t (numRawQSschemaSchemas qs_schema) -> Type)
+                                                               (DelegateImpls : forall idx,
+                                                                   ComputationalADT.pcADT (DelegateSigs idx) (DelegateReps idx))
+                                                               (ValidImpls
+                                                                : forall idx : Fin.t (numRawQSschemaSchemas qs_schema),
+                                                                   refineADT (DelegateSpecs idx)
+                                                                             (ComputationalADT.LiftcADT (existT _ _ (DelegateImpls idx)))),
+                                                               Iterate_Dep_Type_BoundedIndex
+                                                                 (fun idx =>
+                                                                    @refineConstructor _
+                                                                      (cRep' DelegateReps) (cAbsR' _ _ ValidImpls)
+                                                  (consDom (Vector.nth consSigs idx))
+                                                  (getConsDef consDefs idx)
+                                                  (ComputationalADT.LiftcConstructor _ _ (ith  (cCons DelegateReps DelegateImpls) idx))))
+                                                           * (forall
+                                                                 (DelegateReps : Fin.t (numRawQSschemaSchemas qs_schema) -> Type)
+                                                                 (DelegateImpls : forall idx,
+                                                                     ComputationalADT.pcADT (DelegateSigs idx) (DelegateReps idx))
+                                                                 (ValidImpls
+                                                                  : forall idx : Fin.t (numRawQSschemaSchemas qs_schema),
+                                                                     refineADT (DelegateSpecs idx)
+                                                                               (ComputationalADT.LiftcADT (existT _ _ (DelegateImpls idx)))),
+                                                                 Iterate_Dep_Type_BoundedIndex
+                                                                   (fun idx =>
+                                                                      @refineMethod
+                                                                        _ (cRep' DelegateReps)
+                                                                        (cAbsR' _ _ ValidImpls)
+                                                                        (methDom (Vector.nth methSigs idx))
+                                                                        (methCod (Vector.nth methSigs idx))
+                                                                        (getMethDef methDefs idx)
+                                                                        (ComputationalADT.LiftcMethod (ith (cMeths DelegateReps DelegateImpls) idx))))) as ValidRefinements;
+                                                      [ |
+                                                        pose proof (@Notation_Friendly_SharpenFully'
+                                                                      _
+                                                                      _
+                                                                      _
+                                                                      consSigs
+                                                                      methSigs
+                                                                      consDefs
+                                                                      methDefs
+                                                                      _
+                                                                      DelegateSigs
+                                                                      cRep'
+                                                                      cCons
+                                                                      cMeths
+                                                                      DelegateSpecs
+                                                                      cAbsR'
+                                                                      (fst ValidRefinements)
+                                                                      (snd ValidRefinements))
+                                                          as FullySharpenedImpl
+                                                        ; clear ValidRefinements ] ))
+  end;
+    [ simpl; intros; split;
+      [ repeat split; intros; try exact tt;
+        try (etransitivity;
+             [eapply (@Initialize_IndexedQueryStructureImpls_AbsR qs_schema Index)
+             | ];
+             cbv beta;
+             unfold Initialize_IndexedQueryStructureImpls',
+             CallBagImplConstructor; simpl;
+             higher_order_reflexivity
+            )
+      | repeat split; intros; try exact tt;
+        try implement_bag_methods
+      ] | ];
+    simpl in FullySharpenedImpl;
+    fold_string_hyps_in FullySharpenedImpl;
+    fold_heading_hyps_in FullySharpenedImpl;
+    pose_SearchUpdateTerms_in FullySharpenedImpl;
+    pose_search_term_in FullySharpenedImpl;
+    let impl := fresh "impl" in
+    match type of FullySharpenedImpl with
+      @FullySharpenedUnderDelegates _ _ ?Impl =>
+      set (impl := Impl) in *
+    end;
+      cbv beta in *; simpl in impl;
+      let impl' :=
+          match goal with
+            |- @FullySharpenedUnderDelegates _ _ ?Impl => Impl
+          end in
+      (* Not having to worry about re-typing the body during zeta-expansion
+     yields a 30x speedup.
+       *)
+      assert (True) by
+          (clear FullySharpenedImpl; zeta_expand_all impl; unify impl impl'; econstructor);
+        exact FullySharpenedImpl.
+
+Ltac Finish_Master BuildEarlyBag BuildLastBag :=
+    eapply FullySharpened_Finish;
+    [pose_headings_all;
+      match goal with
+      | |- appcontext[ @BuildADT (IndexedQueryStructure ?Schema ?Indexes) ] =>
+        FullySharpenQueryStructure'' Schema Indexes
+      end
+    | simpl; pose_string_ids; pose_headings_all;
+      pose_search_term;  pose_SearchUpdateTerms;
+      match goal with
+        |- context [@Build_IndexedQueryStructure_Impl_Sigs _ ?indices ?SearchTerms _] => try unfold SearchTerms
+      end;
+      BuildQSIndexedBags' BuildEarlyBag BuildLastBag
+    | cbv zeta; pose_string_ids; pose_headings_all;
+      pose_search_term;  pose_SearchUpdateTerms;
+      simpl Sharpened_Implementation;
+      unfold
+        Update_Build_IndexedQueryStructure_Impl_cRep,
+      Join_Comp_Lists',
+      GetIndexedQueryStructureRelation,
+      GetAttributeRaw; simpl;
+      higher_order_reflexivityT ].
+
+Ltac implement_insert' CreateTerm EarlyIndex LastIndex
+     makeClause_dep EarlyIndex_dep LastIndex_dep :=
+        repeat first
+         [simplify with monad laws; simpl
+         | setoid_rewrite refine_If_Then_Else_Bind
+         | match goal with
+             H : DelegateToBag_AbsR ?r_o ?r_n
+             |- context[Pick (fun idx => UnConstrFreshIdx (GetUnConstrRelation ?r_o ?Ridx) idx)] =>
+             let freshIdx := fresh in
+             destruct (exists_UnConstrFreshIdx H Ridx) as [? freshIdx];
+               setoid_rewrite (refine_Pick_UnConstrFreshIdx H Ridx freshIdx)
+           end
+         | etransitivity; [eapply refine_BagADT_QSInsert'; [ eassumption
+                                                           | eauto
+                                                           | intros ] | set_evars ]
+         | implement_Query CreateTerm EarlyIndex LastIndex
+                           makeClause_dep EarlyIndex_dep LastIndex_dep
+         |  setoid_rewrite refine_Pick_DelegateToBag_AbsR; [ | solve [ eauto ] .. ] ].
+
+
+Opaque QSInsert.
+Opaque UpdateUnconstrRelationC.
+
+Definition RosMasterSchema :=
+    Query Structure Schema
+    [
+      relation sNODES has
+               schema <sNODE_ID :: string, sNODE_API :: string>;
+
+      relation sTOPICS has
+                schema <sTOPIC :: string, sTOPIC_TYPE :: string>;
+
+      relation sPARAMS has
+                schema <sKEY :: string, sVALUE :: any>;
+
+      relation sSUBSCRIPTIONS has
+                schema <sNODE_ID :: string, sTOPIC :: string>;
+
+      relation sPARAMSUBSCRIPTIONS has
+                schema <sNODE_ID :: string, sKEY :: string>;
+
+      relation sPUBLICATIONS has
+                schema <sNODE_ID :: string, sTOPIC :: string>;
+
+      relation sSERVICES has
+                schema <sNODE_ID :: string, sSERVICE :: string, sSERVICE_API :: string>
+    ]
+    enforcing [ ].
+
+
+
+Definition RosMasterSpec : ADT _ :=
+  Eval simpl in
+    QueryADTRep RosMasterSchema {
+
+    Def Constructor0 "Init" : rep := empty
+
+    ,
+
+    Def Method4 "registerSubscriber"
+      (r : rep) (caller_id : string) (topic : string) (topic_type : string) (caller_api : string)
+      : rep * (int * string * list string)%type
+      :=
+        res1 <- Insert <sNODE_ID :: caller_id, sTOPIC :: topic> into r ! sSUBSCRIPTIONS;
+
+        if (snd res1) then
+          (res2 <- Insert <sNODE_ID :: caller_id, sNODE_API :: caller_api> into (fst res1) ! sNODES;
+           if (snd res2) then
+             (res3 <- Insert <sTOPIC :: topic, sTOPIC_TYPE :: topic_type> into (fst res2) ! sTOPICS;
+              if snd res3 then
+                (publishers <- For (pub in r ! sPUBLICATIONS) (node in r ! sNODES)
+                            Where ( pub ! sTOPIC = topic  /\  pub ! sNODE_ID = node ! sNODE_ID )
+                            Return ( node ! sNODE_API );
+                 ret(fst res3, (SUCCESS, "You are now subscribed.  Publishers are:", publishers)))
+              else
+                ret(r, (FAILURE, "That topic exists but with a different type.", [])))
+           else
+             ret(r, (FAILURE, "That node exists but with a different api.", [])))
+        else
+          ret(r, (FAILURE, "You are already subscribed to that topic.", []))
+    ,
+
+    Def Method4 "registerPublisher"
+      (r : rep) (caller_id : string) (topic : string) (topic_type : string) (caller_api : string)
+      : rep * (int * string * list string)%type
+      :=
+        res1 <- Insert <sNODE_ID :: caller_id, sTOPIC :: topic> into r ! sPUBLICATIONS;
+        If snd res1 Then
+           (res2 <- Insert <sNODE_ID :: caller_id, sNODE_API :: caller_api> into (fst res1) ! sNODES;
+            If snd res2 Then
+               (res3 <- Insert <sTOPIC :: topic, sTOPIC_TYPE :: topic_type> into (fst res2) ! sTOPICS;
+                If snd res3 Then
+                   subscribers <- For (sub in r ! sSUBSCRIPTIONS) (node in r ! sNODES)
+                   Where ( sub ! sTOPIC = topic  /\  sub ! sNODE_ID = node ! sNODE_ID )
+                   Return ( node ! sNODE_API );
+
+                   ret(fst res3, (SUCCESS, "You are now publishing.  Subscribers are:", subscribers))
+               Else
+               ret(r, (FAILURE, "That topic exists but with a different type.", [])))
+           Else
+           ret(r, (FAILURE, "That node exists but with a different api.", [])))
+           Else
+           ret(r, (FAILURE, "You are already publishing to that topic.", [])),
+
+    Def Method2 "lookupNode"
+      (r : rep) (caller_id : string) (node_name : string)
+      : rep * (int * string * string)%type
+      (* Returns (code, statusMessage, URI) *)
+      :=
+        apis <- For (node in r ! sNODES)
+              Where ( node ! sNODE_ID = node_name )
+              Return ( node ! sNODE_API );
+
+        api <- ret (List.hd "" apis);
+        c <- ret (List.length apis); (* should be either 0 or 1 *)
+
+        if beq_nat c 0 then
+          ret (r, (FAILURE, "Node not found.", api))
+        else
+          ret (r, (SUCCESS, "Node URI is :", api))
+    ,
+
+    Def Method2 "getPublishedTopics"
+      (r : rep) (caller_id : string) (subgraph : string)
+      : rep * (int * string * list (string * string))%type
+      (* Returns (code, statusMessage, [(topic,type)]) *)
+                                                           :=
+        res <- For (topic in r ! sTOPICS) (pub in r ! sPUBLICATIONS)
+            Where ( topic ! sTOPIC = pub ! sTOPIC)
+            Where (stringPrefix topic!sTOPIC subgraph )
+              Return ( (topic ! sTOPIC, topic ! sTOPIC_TYPE) );
+        ret (r, (SUCCESS, "Topics with publishers are :", res))  (* should remove duplicates *)
+    ,
+
+    Def Method1 "getTopicTypes"
+      (r : rep) (caller_id : string)
+      : rep * (int * string * list (string * string))%type
+      :=
+        res <- For (topic in r ! sTOPICS)
+              Return ( (topic ! sTOPIC, topic ! sTOPIC_TYPE) );
+        ret (r, (SUCCESS, "Topics are :", res))
+    ,
+
+    Def Method1 "getSystemState"
+      (r : rep) (caller_id : string)
+      : rep * (int * string * list (list (string * list string)) )%type
+        :=
+        publishers <- For (topic in r ! sTOPICS)
+                 (
+                   pubs <- For (pub in r ! sPUBLICATIONS)
+                             Where (topic ! sTOPIC = pub ! sTOPIC)
+                             Return (pub ! sNODE_ID);
+                   Return ( (topic ! sTOPIC, pubs) )
+                 );
+
+        subscribers <- For (topic in r ! sTOPICS)
+                 (
+                   subs <- For (sub in r ! sSUBSCRIPTIONS)
+                             Where (topic ! sTOPIC = sub ! sTOPIC)
+                             Return (sub ! sNODE_ID);
+                   Return ( (topic ! sTOPIC, subs) )
+                 );
+
+        services <- For (serv in r ! sSERVICES)
+                      Return (serv ! sSERVICE, [serv ! sNODE_ID]);
+
+        ret (r, (SUCCESS, "System state is :", [publishers; subscribers; services]))
+    ,
+
+    Def Method1 "getUri"
+      (r : rep) (caller_id : string)
+      : rep * (int * string * string)%type
+      :=
+        ret (r, (SUCCESS, "My URI is :", "http://localhost:11311"))
+    ,
+
+    Def Method2 "lookupService"
+      (r : rep) (caller_id : string) (service : string)
+      : rep * (int * string * string)%type
+      :=
+        ids <- For (serv in r ! sSERVICES)
+              Where ( serv ! sSERVICE = service )
+              Return ( serv ! sNODE_ID );
+
+        id <- ret (List.hd "" ids);
+        c <- ret (List.length ids); (* should be either 0 or 1 *)
+
+        if beq_nat c 0 then (* could use 'match ... with' instead of if *)
+          ret (r, (FAILURE, "No one is provind that service.", id))
+        else
+          ret (r, (SUCCESS, "Service provider is :", id))
+
+}%methDefParsing.
+
+(*raise_error.
+
+Set Ltac Debug.
+*)
+
+Theorem SharpenedRosMaster :
+  FullySharpened RosMasterSpec.
+Proof.
+  unfold RosMasterSpec.
+  pose_string_hyps.
+  start sharpening ADT.
+  eapply SharpenStep;
+  [ match goal with
+        |- context [@BuildADT (QueryStructure ?Rep) _ _ _ _ _ _] =>
+        eapply refineADT_BuildADT_Rep_refine_All with (AbsR := @DropQSConstraints_AbsR Rep);
+          [ repeat (first [eapply refine_Constructors_nil
+                          | eapply refine_Constructors_cons;
+                            [ simpl; intros;
+                              match goal with
+                              | |- refine _ (?E _ _ _ _) => let H := fresh in set (H := E)
+                              | |- refine _ (?E _ _ _) => let H := fresh in set (H := E)
+                              | |- refine _ (?E _ _) => let H := fresh in set (H := E)
+                              | |- refine _ (?E _) => let H := fresh in set (H := E)
+                              | |- refine _ (?E) => let H := fresh in set (H := E)
+                              | _ => idtac
+                              end;
+                              (* Drop constraints from empty *)
+                              try apply Constructor_DropQSConstraints;
+                              cbv delta [GetAttribute] beta; simpl
+                            | ] ])
+          | repeat (first [eapply refine_Methods_nil
+                          | eapply refine_Methods_cons;
+                            [ simpl; intros;
+                              match goal with
+                              | |- refine _ (?E _ _ _ _) => let H := fresh in set (H := E)
+                              | |- refine _ (?E _ _ _) => let H := fresh in set (H := E)
+                              | |- refine _ (?E _ _) => let H := fresh in set (H := E)
+                              | |- refine _ (?E _) => let H := fresh in set (H := E)
+                              | |- refine _ (?E) => let H := fresh in set (H := E)
+                              | _ => idtac
+                              end;
+                              cbv delta [GetAttribute] beta; simpl | ]
+                          ])]
+    end | ].
+  - simplify with monad laws.
+    etransitivity.
+    eapply QSInsertSpec_refine_subgoals; try eassumption; set_evars.
+    + rewrite decides_True; finish honing.
+    + simpl. refine pick val true; simpl; eauto; finish honing.
+    + simpl. intros; refine pick val true; simpl; eauto; finish honing.
+    + simpl. repeat foreignToQuery'. finish honing.
+    + simpl. intros; finish honing.
+    + simpl; intros; simplify with monad laws.
+      etransitivity.
+      eapply QSInsertSpec_refine_subgoals; try eassumption; set_evars.
+      * simpl; rewrite decides_True; finish honing.
+      * simpl. refine pick val true; simpl; eauto; finish honing.
+      * simpl. intros; refine pick val true; simpl; eauto; finish honing.
+      * simpl. repeat foreignToQuery'. finish honing.
+      * simpl. intros; repeat (remove_trivial_fundep_insertion_constraints; simpl).
+        finish honing.
+      * simpl; intros; simplify with monad laws.
+        etransitivity.
+        { eapply QSInsertSpec_refine_subgoals; try eassumption; set_evars.
+          * simpl; rewrite decides_True; finish honing.
+          * simpl. refine pick val true; simpl; eauto; finish honing.
+          * simpl. intros; refine pick val true; simpl; eauto; finish honing.
+          * simpl. repeat foreignToQuery'. finish honing.
+          * simpl. intros; repeat (remove_trivial_fundep_insertion_constraints; simpl).
+            finish honing.
+          * simpl; intros.
+            simplify with monad laws; cbv beta; simpl.
+            drop_constraints_from_query.
+          * intros; simpl; simplify with monad laws.
+            simpl; refine pick val _; try eassumption.
+            simplify with monad laws; finish honing.
+        }
+        simplify with monad laws.
+        repeat setoid_rewrite refine_if_Then_Else_Duplicate.
+        finish honing.
+      * intros; simpl; simplify with monad laws.
+        simpl; refine pick val _; try eassumption.
+        simplify with monad laws; finish honing.
+      * intros; simpl; simplify with monad laws.
+        repeat setoid_rewrite refine_if_Then_Else_Duplicate.
+        finish honing.
+    + intros; simpl; simplify with monad laws.
+      simpl; refine pick val _; try eassumption.
+      simplify with monad laws; finish honing.
+    + intros; simpl; simplify with monad laws.
+      finish honing.
+  - simplify with monad laws.
+    etransitivity.
+    eapply QSInsertSpec_refine_subgoals; try eassumption; set_evars.
+    + rewrite decides_True; finish honing.
+    + simpl. refine pick val true; simpl; eauto; finish honing.
+    + simpl. intros; refine pick val true; simpl; eauto; finish honing.
+    + simpl. repeat foreignToQuery'. finish honing.
+    + simpl. intros; finish honing.
+    + simpl; intros; simplify with monad laws.
+      etransitivity.
+      eapply QSInsertSpec_refine_subgoals; try eassumption; set_evars.
+      * simpl; rewrite decides_True; finish honing.
+      * simpl. refine pick val true; simpl; eauto; finish honing.
+      * simpl. intros; refine pick val true; simpl; eauto; finish honing.
+      * simpl. repeat foreignToQuery'. finish honing.
+      * simpl. intros; repeat (remove_trivial_fundep_insertion_constraints; simpl).
+        finish honing.
+      * simpl; intros; simplify with monad laws.
+        etransitivity.
+        { eapply QSInsertSpec_refine_subgoals; try eassumption; set_evars.
+          * simpl; rewrite decides_True; finish honing.
+          * simpl. refine pick val true; simpl; eauto; finish honing.
+          * simpl. intros; refine pick val true; simpl; eauto; finish honing.
+          * simpl. repeat foreignToQuery'. finish honing.
+          * simpl. intros; repeat (remove_trivial_fundep_insertion_constraints; simpl).
+            finish honing.
+          * simpl; intros.
+            simplify with monad laws; cbv beta; simpl.
+            drop_constraints_from_query.
+          * intros; simpl; simplify with monad laws.
+            simpl; refine pick val _; try eassumption.
+            simplify with monad laws; finish honing.
+        }
+        simplify with monad laws.
+        repeat setoid_rewrite refine_if_Then_Else_Duplicate.
+        finish honing.
+      * intros; simpl; simplify with monad laws.
+        simpl; refine pick val _; try eassumption.
+        simplify with monad laws; finish honing.
+      * intros; simpl; simplify with monad laws.
+        repeat setoid_rewrite refine_if_Then_Else_Duplicate.
+        finish honing.
+    + intros; simpl; simplify with monad laws.
+      simpl; refine pick val _; try eassumption.
+      simplify with monad laws; finish honing.
+    + intros; simpl; simplify with monad laws.
+      finish honing.
+  - drop_constraints_from_query.
+  - drop_constraints_from_query.
+  - drop_constraints_from_query.
+  - drop_constraints_from_query.
+  - drop_constraints_from_query.
+  - drop_constraints_from_query.
+  - GenerateIndexesForAll
+   EqExpressionAttributeCounter
+   ltac:(fun attrlist =>
+           let attrlist' := eval compute in (PickIndexes _ (CountAttributes' attrlist)) in make_simple_indexes attrlist'
+                                                                                                               ltac:(LastCombineCase6 BuildEarlyEqualityIndex)
+                                                                                                                      ltac:(LastCombineCase5 BuildLastEqualityIndex)).
+    + plan EqIndexUse createEarlyEqualityTerm createLastEqualityTerm
+           EqIndexUse_dep createEarlyEqualityTerm_dep createLastEqualityTerm_dep.
+    + implement_insert' EqIndexUse createEarlyEqualityTerm createLastEqualityTerm
+                        EqIndexUse_dep createEarlyEqualityTerm_dep createLastEqualityTerm_dep;
+      doAny ltac:(implement_insert'
+                    EqIndexUse createEarlyEqualityTerm createLastEqualityTerm
+                    EqIndexUse_dep createEarlyEqualityTerm_dep createLastEqualityTerm_dep)
+                   rewrite_drill ltac:(finish honing).
+    + implement_insert' EqIndexUse createEarlyEqualityTerm createLastEqualityTerm
+                        EqIndexUse_dep createEarlyEqualityTerm_dep createLastEqualityTerm_dep;
+      doAny ltac:(implement_insert'
+                    EqIndexUse createEarlyEqualityTerm createLastEqualityTerm
+                    EqIndexUse_dep createEarlyEqualityTerm_dep createLastEqualityTerm_dep)
+                   rewrite_drill ltac:(finish honing).
+    + plan EqIndexUse createEarlyEqualityTerm createLastEqualityTerm
+           EqIndexUse_dep createEarlyEqualityTerm_dep createLastEqualityTerm_dep.
+    + plan EqIndexUse createEarlyEqualityTerm createLastEqualityTerm
+           EqIndexUse_dep createEarlyEqualityTerm_dep createLastEqualityTerm_dep.
+    + plan EqIndexUse createEarlyEqualityTerm createLastEqualityTerm
+           EqIndexUse_dep createEarlyEqualityTerm_dep createLastEqualityTerm_dep.
+    + implement_nested_Query EqIndexUse createEarlyEqualityTerm createLastEqualityTerm
+                             EqIndexUse_dep createEarlyEqualityTerm_dep createLastEqualityTerm_dep.
+      implement_nested_Query EqIndexUse createEarlyEqualityTerm createLastEqualityTerm
+                             EqIndexUse_dep createEarlyEqualityTerm_dep createLastEqualityTerm_dep.
+      implement_Query EqIndexUse createEarlyEqualityTerm createLastEqualityTerm
+                      EqIndexUse_dep createEarlyEqualityTerm_dep createLastEqualityTerm_dep.
+      simplify with monad laws.
+      cbv beta; simpl; commit.
+      finish honing.
+    + simplify with monad laws; simpl.
+      refine pick val _; eauto.
+      simplify with monad laws.
+      finish honing.
+    + plan EqIndexUse createEarlyEqualityTerm createLastEqualityTerm
+           EqIndexUse_dep createEarlyEqualityTerm_dep createLastEqualityTerm_dep.
+    + Finish_Master BuildEarlyBag BuildLastBag.
+Time Defined.
+
+
+Time Definition ROSMasterImpl : ComputationalADT.cADT _ :=
+  Eval simpl in projT1 SharpenedRosMaster.
+
+Print BookstoreImpl.
