src/QueryStructure/Automation/Constraints/ForeignKeyAutomation.v
@@ -17,15 +17,30 @@ Require Import Coq.Lists.List Coq.Arith.Compare_dec Coq.Bool.Bool Coq.Strings.St
         Fiat.QueryStructure.Automation.Common.
 
 Ltac foreignToQuery :=
-      match goal with
-    | [ |- context[{ b' | decides b' (ForeignKey_P ?AttrID ?AttrID' ?tupmap ?n (@GetUnConstrRelation ?qs_schema ?or ?TableID))}] ]
-      =>
-      let H' := fresh in
-      let H' :=
-      eval simpl in (@refine_constraint_check_into_query
-                       qs_schema TableID
-                       (fun tup : RawTuple => GetAttributeRaw n AttrID = tupmap (GetAttributeRaw tup AttrID')) or _) in
-          pose_string_hyps; pose_heading_hyps;
-                    (* fold_string_hyps_in H'; fold_heading_hyps_in H'; *)
-                    setoid_rewrite H'; simplify with monad laws; cbv beta; simpl
+  match goal with
+  | [ |- context[{ b' | decides b' (ForeignKey_P ?AttrID ?AttrID' ?tupmap ?n (@GetUnConstrRelation ?qs_schema ?or ?TableID))}] ]
+    =>
+    let H' := fresh in
+    let H' :=
+        eval simpl in (@refine_constraint_check_into_query
+                         qs_schema TableID
+                         (fun tup : RawTuple => GetAttributeRaw n AttrID = tupmap (GetAttributeRaw tup AttrID')) or _) in
+        pose_string_hyps; pose_heading_hyps;
+                      (* fold_string_hyps_in H'; fold_heading_hyps_in H'; *)
+                      setoid_rewrite H'; simplify with monad laws; cbv beta; simpl
+  end.
+
+Ltac foreignToQuery' :=
+  match goal with
+  | [ |- context[{ b' | decides b' (@ForeignKey_P ?heading ?relSchema ?AttrID ?AttrID' ?tupmap ?n (@GetUnConstrRelation ?qs_schema ?or ?TableID))}] ]
+    =>
+    let H' := fresh in
+    let H' :=
+        eval simpl in
+    (@refine_constraint_check_into_query
+       qs_schema TableID
+       (fun tup : @RawTuple heading => @GetAttributeRaw heading n AttrID = tupmap (@GetAttributeRaw relSchema tup AttrID')) or _) in
+        pose_string_hyps; pose_heading_hyps;
+    (* fold_string_hyps_in H'; fold_heading_hyps_in H'; *)
+    setoid_rewrite H'; try simplify with monad laws; cbv beta; simpl
   end.
