src/QueryStructure/Automation/Constraints/FunctionalDependencyAutomation.v
@@ -22,21 +22,21 @@ Require Import Coq.Lists.List
         Fiat.QueryStructure.Automation.Common.
 
 Ltac dec_tauto :=
-    clear; intuition eauto;
-    eapply Tuple_Agree_eq_dec;
-    match goal with
-      | [ |- ?E = true ] => case_eq E; intuition idtac; [ exfalso ]
-    end;
-    match goal with
-      | [ H : _ |- _ ] => apply Tuple_Agree_eq_dec' in H; solve [ eauto ]
-    end.
+  clear; intuition eauto;
+  eapply Tuple_Agree_eq_dec;
+  match goal with
+  | [ |- ?E = true ] => case_eq E; intuition idtac; [ exfalso ]
+  end;
+  match goal with
+  | [ H : _ |- _ ] => apply Tuple_Agree_eq_dec' in H; solve [ eauto ]
+  end.
 
-  Lemma query_eq_true_iff {A}
-        (q_eq : Query_eq A)
-    : forall (a a' : A), ?[ A_eq_dec a a'] = true <-> a = a'.
-  Proof.
-    intros; destruct (A_eq_dec a a'); split; intros; try congruence.
-  Qed.
+Lemma query_eq_true_iff {A}
+      (q_eq : Query_eq A)
+  : forall (a a' : A), ?[ A_eq_dec a a'] = true <-> a = a'.
+Proof.
+  intros; destruct (A_eq_dec a a'); split; intros; try congruence.
+Qed.
 
 Ltac prove_decidability_for_functional_dependencies :=
   simpl; econstructor; intros;
@@ -57,77 +57,113 @@ Ltac prove_decidability_for_functional_dependencies :=
 Hint Extern 100 (DecideableEnsemble _) => prove_decidability_for_functional_dependencies : typeclass_instances.
 
 Tactic Notation "refine" "existence" "check" "into" "query" :=
-      match goal with
-          |- context[{b | decides b
-                                  (exists tup : @IndexedTuple ?heading,
-                                     (@GetUnConstrRelation ?qs_schema ?qs ?tbl tup /\ @?P tup))}]
-          =>
-          let H1 := fresh in
-          let H2 := fresh in
-            makeEvar (Ensemble (@Tuple heading))
-                     ltac:(fun P' => assert (Same_set (@IndexedTuple heading) (fun t => P' (indexedElement t)) P) as H1;
-            [unfold Same_set, Included, Ensembles.In;
-              split; [intros x H; pattern (indexedElement x);
-                      match goal with
-                          |- ?P'' (indexedElement x) => unify P' P'';
-                            simpl; eauto
-                      end
-                     | eauto]
-            |
-            assert (DecideableEnsemble P') as H2;
-              [ simpl; eauto with typeclass_instances (* Discharge DecideableEnsemble w/ intances. *)
-              | setoid_rewrite (@refine_constraint_check_into_query' qs_schema tbl qs P P' H2 H1); clear H1 H2 ] ]) end.
+  match goal with
+    |- context[{b | decides b
+                            (exists tup : @IndexedTuple ?heading,
+                                (@GetUnConstrRelation ?qs_schema ?qs ?tbl tup /\ @?P tup))}]
+    =>
+    let H1 := fresh in
+    let H2 := fresh in
+    makeEvar (Ensemble (@Tuple heading))
+             ltac:(fun P' => assert (Same_set (@IndexedTuple heading) (fun t => P' (indexedElement t)) P) as H1;
+                   [unfold Same_set, Included, Ensembles.In;
+                     split; [intros x H; pattern (indexedElement x);
+                             match goal with
+                               |- ?P'' (indexedElement x) => unify P' P'';
+                                 simpl; eauto
+                             end
+                            | eauto]
+                   |
+                   assert (DecideableEnsemble P') as H2;
+                     [ simpl; eauto with typeclass_instances (* Discharge DecideableEnsemble w/ intances. *)
+                     | setoid_rewrite (@refine_constraint_check_into_query' qs_schema tbl qs P P' H2 H1); clear H1 H2 ] ]) end.
+
+Ltac funDepToQuery :=
+  match goal with
+  | |-
+    context [{b : _ |
+              decides b
+                      (forall tup' : @IndexedElement ?T,
+                          GetUnConstrRelation (QSSchema := ?qsSchema) ?or ?Ridx _ ->
+                          @FunctionalDependency_P ?heading ?attrlist1 ?attrlist2 ?n _)}] =>
+    let H' := fresh in
+    let H'' := fresh in
+    let refine_fundep := fresh in
+    assert
+      ((forall (tup' : @IndexedElement T),
+           GetUnConstrRelation or Ridx tup' ->
+           @FunctionalDependency_P heading attrlist1 attrlist2 n (indexedElement tup')) <->
+       (forall tup' : @IndexedElement T,
+           ~
+             (GetUnConstrRelation or Ridx tup' /\
+              @tupleAgree heading n (indexedElement tup') attrlist2 /\
+              ~ @tupleAgree heading n (indexedElement tup') attrlist1)))
+      as H' by (unfold FunctionalDependency_P; dec_tauto);
+      assert
+        (DecideableEnsemble
+           (fun x : T =>
+              @tupleAgree_computational heading n x attrlist2 /\
+              ~ @tupleAgree_computational heading n x attrlist1))
+      as H''
+        by (subst_all;
+            FunctionalDependencyAutomation.prove_decidability_for_functional_dependencies);
+      (let refine_fundep :=
+           eval simpl in
+       ( (@refine_functional_dependency_check_into_query qsSchema Ridx n attrlist2
+                                                         attrlist1 or H'' H')) in
+           setoid_rewrite refine_fundep; clear H'' H')
+  end.
 
 Ltac fundepToQuery :=
   match goal with
-    | [ |- context[Pick
-                     (fun b => decides
-                                 b
-                                 (forall tup' : @IndexedRawTuple ?sch,
-                                     GetUnConstrRelation (QSSchema := ?qs_schema) ?or ?Ridx _
-                                     -> @FunctionalDependency_P ?heading ?attrlist1 ?attrlist2 ?n _))] ] =>
-      let H' := fresh in
-      let H'' := fresh in
-      let refine_fundep := fresh in
-      assert ((forall tup' : IndexedRawTuple,
-                 GetUnConstrRelation or Ridx tup'
-                 -> @FunctionalDependency_P heading attrlist1 attrlist2 n (indexedElement tup'))
-              <-> (forall tup' : IndexedRawTuple,
-                     ~ (GetUnConstrRelation or Ridx tup'
-                        /\ @tupleAgree sch n (indexedElement tup') attrlist2
-                        /\ ~ @tupleAgree sch n (indexedElement tup') attrlist1))) as H'
-          by (unfold FunctionalDependency_P; dec_tauto);
-        assert (DecideableEnsemble (fun x : RawTuple =>
-                                      @tupleAgree_computational sch n x attrlist2 /\
-                                      ~ @tupleAgree_computational sch n x attrlist1)) as H''
-          by (subst_all;
-              prove_decidability_for_functional_dependencies);
-        let refine_fundep := eval simpl in (@refine_functional_dependency_check_into_query qs_schema Ridx n attrlist2 attrlist1 or H'' H') in
+  | [ |- context[Pick
+                   (fun b => decides
+                               b
+                               (forall tup' : @IndexedRawTuple ?sch,
+                                   GetUnConstrRelation (QSSchema := ?qs_schema) ?or ?Ridx _
+                                   -> @FunctionalDependency_P ?heading ?attrlist1 ?attrlist2 ?n _))] ] =>
+    let H' := fresh in
+    let H'' := fresh in
+    let refine_fundep := fresh in
+    assert ((forall tup' : IndexedRawTuple,
+                GetUnConstrRelation or Ridx tup'
+                -> @FunctionalDependency_P heading attrlist1 attrlist2 n (indexedElement tup'))
+            <-> (forall tup' : IndexedRawTuple,
+                    ~ (GetUnConstrRelation or Ridx tup'
+                       /\ @tupleAgree sch n (indexedElement tup') attrlist2
+                       /\ ~ @tupleAgree sch n (indexedElement tup') attrlist1))) as H'
+        by (unfold FunctionalDependency_P; dec_tauto);
+      assert (DecideableEnsemble (fun x : RawTuple =>
+                                    @tupleAgree_computational sch n x attrlist2 /\
+                                    ~ @tupleAgree_computational sch n x attrlist1)) as H''
+        by (subst_all;
+            prove_decidability_for_functional_dependencies);
+      let refine_fundep := eval simpl in (@refine_functional_dependency_check_into_query qs_schema Ridx n attrlist2 attrlist1 or H'' H') in
           (* as refine_fundep; simpl in refine_fundep;
         fold_heading_hyps_in refine_fundep; fold_string_hyps_in refine_fundep; *)
-        setoid_rewrite refine_fundep; clear H'' H'
-    | [ |- context[Pick
-                     (fun b => decides
-                                 b
-                                 (forall tup' : @IndexedRawTuple ?sch,
-                                     GetUnConstrRelation ?or ?Ridx _
-                                     -> @FunctionalDependency_P ?heading ?attrlist1 ?attrlist2 _ ?n ))] ] =>
-      let H' := fresh in
-      let H'' := fresh in
-      let refine_fundep := fresh in
-      assert ((forall tup' : IndexedTuple,
-                 GetUnConstrRelation or Ridx tup'
-                 -> @FunctionalDependency_P heading attrlist1 attrlist2 (indexedElement tup') n)
-              <-> (forall tup' : IndexedTuple,
-                     ~ (GetUnConstrRelation or Ridx tup'
-                        /\ @tupleAgree sch (indexedElement tup') n attrlist2
-                        /\ ~ @tupleAgree sch (indexedElement tup') n attrlist1))) as H'
-          by (unfold FunctionalDependency_P; dec_tauto);
-        assert (DecideableEnsemble (fun x : Tuple =>
-                                      @tupleAgree_computational sch x n attrlist2 /\
-                                      ~ @tupleAgree_computational sch x n attrlist1)) as H''
-          by prove_decidability_for_functional_dependencies;
-        let refine_fundep := eval simpl in
-        (@refine_functional_dependency_check_into_query' _ _ n attrlist2 attrlist1 or H'' H') in
-            (*simpl in refine_fundep; setoid_rewrite refine_fundep; *) clear H'' H'
+          setoid_rewrite refine_fundep; clear H'' H'
+  | [ |- context[Pick
+                   (fun b => decides
+                               b
+                               (forall tup' : @IndexedRawTuple ?sch,
+                                   GetUnConstrRelation ?or ?Ridx _
+                                   -> @FunctionalDependency_P ?heading ?attrlist1 ?attrlist2 _ ?n ))] ] =>
+    let H' := fresh in
+    let H'' := fresh in
+    let refine_fundep := fresh in
+    assert ((forall tup' : IndexedTuple,
+                GetUnConstrRelation or Ridx tup'
+                -> @FunctionalDependency_P heading attrlist1 attrlist2 (indexedElement tup') n)
+            <-> (forall tup' : IndexedTuple,
+                    ~ (GetUnConstrRelation or Ridx tup'
+                       /\ @tupleAgree sch (indexedElement tup') n attrlist2
+                       /\ ~ @tupleAgree sch (indexedElement tup') n attrlist1))) as H'
+        by (unfold FunctionalDependency_P; dec_tauto);
+      assert (DecideableEnsemble (fun x : Tuple =>
+                                    @tupleAgree_computational sch x n attrlist2 /\
+                                    ~ @tupleAgree_computational sch x n attrlist1)) as H''
+        by prove_decidability_for_functional_dependencies;
+      let refine_fundep := eval simpl in
+      (@refine_functional_dependency_check_into_query' _ _ n attrlist2 attrlist1 or H'' H') in
+          (*simpl in refine_fundep; setoid_rewrite refine_fundep; *) clear H'' H'
   end; try simplify with monad laws; pose_string_hyps; pose_heading_hyps.
